C11-BackEnds/Clean/src/Clean.thy
@@ -1410,6 +1410,11 @@ fun mk_seq_C C C' = let val t = fastype_of C
                      val t' =  fastype_of C'
                  in  Const(\<^const_name>\<open>bind_SE'\<close>, t --> t' --> t') $ C $ C' end;
 
+fun mk_seq_assign_C rhs lhs varname vartyp= let
+                    val t1 = fastype_of rhs
+                    val t2 = fastype_of lhs
+                in Const(\<^const_name>\<open>bind_SE\<close>, t1 --> (vartyp --> t2) --> t2 ) $ rhs $ (Abs (varname,vartyp, lhs)) end;
+
 fun mk_skip_C sty = Const(\<^const_name>\<open>skip\<^sub>S\<^sub>E\<close>, StateMgt_core.MON_SE_T HOLogic.unitT sty)
 
 fun mk_break sty = 
